Tealeaves/Examples/LambdaNominal/Demo.v
@@ -1,34 +1,78 @@
+From Tealeaves Require Export
+  Examples.LambdaNominal.Categorical
+  Backends.Named.FV
+  Backends.Named.Barendregt
+  Backends.Adapters.NamedToLN.
 
-Require Import Coq.Arith.Wf_nat.
+Import LambdaNominal.Syntax.Notations.
 
-Definition nat_lt (x y : nat) := x < y.
-
-Lemma nat_lt_wf : well_founded nat_lt.
-Proof.
-  unfold well_founded.
-  intros n.
-  induction n as [|n' IH].
-  - (* Base case: 0 is accessible because there are no smaller numbers *)
-    constructor. intros y Hy. inversion Hy.
-  - (* Inductive step: every smaller number is accessible *)
-    constructor. intros y Hy.
-    apply IH.
-    unfold nat_lt in *.
-    admit.
-Admitted.
-
-Lemma lt_succ_diag_r : forall n, n < S n.
-Proof.
-  intros. auto.
-Qed.
+From Tealeaves Require Export
+  Classes.Categorical.DecoratedTraversableFunctorPoly
+  Classes.Kleisli.DecoratedTraversableMonadPoly.
 
 
-About Acc.
-Print Acc.
-Fixpoint fact (n : nat) (Hn : Acc nat_lt n) : nat :=
-  match n as n' return (Acc nat_lt n' -> nat) with
-  | 0 => fun _ => 1
-  | S n' => fun Hn =>
-      let Hn' := match Hn with Acc_intro _ Hacc => Hacc n' (lt_succ_diag_r n') end in
-      (S n') * fact n' Hn'
-  end Hn.
+From Tealeaves Require
+  Adapters.MonoidHom.DecoratedTraversableMonad
+  Adapters.PolyToMono.Kleisli.DecoratedFunctor
+  Adapters.PolyToMono.Kleisli.DecoratedTraversableFunctor
+  Adapters.PolyToMono.Kleisli.DecoratedTraversableMonad
+  Adapters.CategoricalToKleisli.DecoratedTraversableMonadPoly
+  Adapters.CategoricalToKleisli.TraversableFunctor
+  Adapters.CategoricalToKleisli.DecoratedTraversableFunctor.
+
+
+Import Kleisli.DecoratedFunctorPoly.
+Import CategoricalToKleisli.DecoratedFunctorPoly.
+Import CategoricalToKleisli.DecoratedFunctorPoly.DerivedOperations.
+Import CategoricalToKleisli.DecoratedFunctorPoly.DerivedInstances.
+Import CategoricalToKleisli.DecoratedTraversableFunctorPoly.DerivedOperations.
+Import CategoricalToKleisli.DecoratedTraversableFunctorPoly.DerivedInstances.
+Import CategoricalToKleisli.DecoratedTraversableMonadPoly.DerivedOperations.
+Import CategoricalToKleisli.DecoratedTraversableMonadPoly.DerivedInstances.
+
+Import DecoratedFunctorPoly.ToMono.
+Import TraversableFunctor2.ToMono.
+Import PolyToMono.Kleisli.DecoratedFunctor.ToMono1.
+
+Import CategoricalToKleisli.TraversableFunctor.DerivedOperations.
+Import CategoricalToKleisli.TraversableFunctor.DerivedInstances.
+
+Import CategoricalToKleisli.DecoratedTraversableFunctor.DerivedOperations.
+Import CategoricalToKleisli.DecoratedTraversableFunctor.DerivedInstances.
+
+Existing Instance Theory.DecoratedTraversableFunctor.ToCtxset_Mapdt.
+Existing Instance Theory.TraversableFunctor.ToSubset_Traverse.
+
+
+
+
+Example term0 := (λ 0, `0).
+Example term1 := (λ 1, `1 · `2).
+Example term2 := (λ 0, `1 · `0).
+Example term3 := (λ 2, `1 · `0).
+Example term4 := (λ 2, `1 · `2).
+Example term5 := (λ 2, `10 · `2).
+
+Compute FV term0.
+Compute FV term1.
+Compute FV term2.
+Compute FV term3.
+Compute FV term4.
+Compute FV term5.
+
+Compute subst 0 term0 term0. (* (λ) 1 `1 *)
+Compute subst 0 term1 term0. (* (λ) 1 `1 *)
+Compute subst 0 term2 term0. (* (λ) 2 `2 *)
+Compute subst 0 term3 term0. (* (λ) 2 `2 *)
+Compute subst 0 term4 term0. (* (λ) 2 `2 *)
+Compute subst 0 term5 term0. (* (λ) 1 `1 *)
+
+Compute subst 0 term0 term1.
+Compute subst 0 term1 term1.
+Compute subst 0 term2 term1.
+Compute subst 0 term4 term1.
+Compute subst 0 term5 term1.
+
+Compute term_nominal_to_ln term term0.
+Compute term_nominal_to_ln term term1.
+Compute term_nominal_to_ln term term5.
